proof: add note about AssocLookup

cogent/isa/AssocLookup.thy
@@ -40,6 +40,28 @@ lemma assoc_lookup_simps[simp]:
 declare assoc_lookup.simps[simp del]
 
 (*
+XXX: the Isabelle code for this was changed to return option, but the ML code below wasn't changed.
+You need to use the ML code to get any benefit from this representation, as it adds a separate simp for each element.
+
+
+fun assoc_lookup :: "('a \<times> 'b) list \<Rightarrow> 'b \<Rightarrow> 'a \<Rightarrow> 'b" where
+    "assoc_lookup [] def _ = def"
+  | "assoc_lookup ((k, v) # ls) def x = (if x = k then v else assoc_lookup ls def x)"
+
+(* These versions are better for simp performance *)
+lemma assoc_lookup_simps[simp]:
+  "assoc_lookup [] def x = def"
+  "assoc_lookup ((k, v) # ls) def k = v"
+  (* make_assoc_fun shouldn't need this one *)
+  (*"x = k \<Longrightarrow> assoc_lookup ((k, v) # ls) def x = v"*)
+  "x \<noteq> k \<Longrightarrow> assoc_lookup ((k, v) # ls) def x = assoc_lookup ls def x"
+  by simp_all
+declare assoc_lookup.simps[simp del]
+
+*)
+
+
+(*
  * Main interface.
  * Note that all types in "assocs" and "default" need to match,
  * this procedure doesn't do type unification. *)
